ulib/FStar.Tactics.Builtins.fsti
@@ -397,3 +397,8 @@ val term_to_string : term -> Tac string
 (** Print a computation type via the pretty printer. See comment
 on [term_to_string]. *)
 val comp_to_string : comp -> Tac string
+
+(** A variant of Reflection.term_eq that may inspect more underlying
+details of terms. This function could distinguish two _otherwise equal
+terms_, but that distinction cannot leave the Tac effect. *)
+val term_eq' : term -> term -> Tac bool
